cequiv/cequiv_bind.v
@@ -1,0 +1,530 @@
+(*
+
+  Copyright 2014 Cornell University
+  Copyright 2015 Cornell University
+
+  This file is part of VPrl (the Verified Nuprl project).
+
+  VPrl is free software: you can redistribute it and/or modify
+  it under the terms of the GNU General Public License as published by
+  the Free Software Foundation, either version 3 of the License, or
+  (at your option) any later version.
+
+  VPrl is distributed in the hope that it will be useful,
+  but WITHOUT ANY WARRANTY; without even the implied warranty of
+  MERCHANTABILITY or FITNESS FOR A PARTICULAR PURPOSE.  See the
+  GNU General Public License for more details.
+
+  You should have received a copy of the GNU General Public License
+  along with VPrl.  If not, see <http://www.gnu.org/licenses/>.
+
+
+  Website: http://nuprl.org/html/verification/
+  Authors: Abhishek Anand & Vincent Rahli
+
+ *)
+
+
+Require Export cequiv.
+Require Export csubst2.
+
+
+Definition pv_olift {o} (R : NTrel) (x y : @NTerm o) vs : [univ] :=
+  forall sub: Sub,
+    prog_sub sub
+    -> dom_sub sub = vs
+    -> R (lsubst x sub) (lsubst y sub).
+
+Definition sub_find_def {o} (sub : @Sub o) v d : NTerm :=
+  match sub_find sub v with
+    | Some t => t
+    | None => d
+  end.
+
+Fixpoint sub_select {o} (sub : @Sub o) (vars : list NVar) (d : NTerm) : Sub :=
+  match vars with
+    | nil => nil
+    | v :: vs => (v,sub_find_def sub v d) :: sub_select sub vs d
+  end.
+
+Lemma dom_sub_sub_select {o} :
+  forall (s : @Sub o) d vs,
+    dom_sub (sub_select s vs d) = vs.
+Proof.
+  induction vs; introv; allsimpl; tcsp.
+  rw IHvs; auto.
+Qed.
+
+Definition eq_option {o} (op1 op2 : option (@NTerm o)) :=
+  match op1, op2 with
+    | Some t1, Some t2 => t1 = t2
+    | None, None => True
+    | _,_ => False
+  end.
+
+Definition ext_eq_subs {o} vs (sub1 sub2 : @Sub o) :=
+  forall v,
+    LIn v vs
+    -> eq_option (sub_find sub1 v) (sub_find sub2 v).
+
+Lemma eq_lsubst_aux_if_ext_eq {o} :
+  forall (t : @NTerm o) sub1 sub2,
+    ext_eq_subs (free_vars t) sub1 sub2
+    -> disjoint (bound_vars t) (sub_free_vars sub1)
+    -> disjoint (bound_vars t) (sub_free_vars sub2)
+    -> lsubst_aux t sub1 = lsubst_aux t sub2.
+Proof.
+  nterm_ind1s t as [v|f|op bs ind] Case; introv ext d1 d2; allsimpl; auto.
+
+  - Case "vterm".
+    pose proof (ext v) as h.
+    remember (sub_find sub1 v) as sf1; symmetry in Heqsf1; destruct sf1;
+    remember (sub_find sub2 v) as sf2; symmetry in Heqsf2; destruct sf2;
+    allsimpl; tcsp.
+
+  - Case "oterm".
+    f_equal.
+    apply eq_maps; introv i.
+    destruct x as [l t].
+    allsimpl.
+    f_equal.
+
+    pose proof (ind t t l i) as h; clear ind.
+    autodimp h hyp; eauto 3 with slow.
+    apply h.
+
+    + introv j.
+      allrw @sub_find_sub_filter_eq.
+      destruct (in_deq _ deq_nvar v l) as [d|d]; boolvar; tcsp; GC.
+      apply ext.
+      rw lin_flat_map.
+      eexists; dands; eauto.
+      simpl.
+      rw in_remove_nvars; sp.
+
+    + introv j k.
+      pose proof (d1 t0) as q.
+      autodimp q hyp.
+      { rw lin_flat_map.
+        eexists; dands; eauto.
+        simpl.
+        rw in_app_iff; sp. }
+      apply subset_sub_free_vars_sub_filter in k; sp.
+
+    + introv j k.
+      pose proof (d2 t0) as q.
+      autodimp q hyp.
+      { rw lin_flat_map.
+        eexists; dands; eauto.
+        simpl.
+        rw in_app_iff; sp. }
+      apply subset_sub_free_vars_sub_filter in k; sp.
+Qed.
+
+Lemma cl_eq_lsubst_if_ext_eq {o} :
+  forall (t : @NTerm o) sub1 sub2,
+    cl_sub sub1
+    -> cl_sub sub2
+    -> ext_eq_subs (free_vars t) sub1 sub2
+    -> lsubst t sub1 = lsubst t sub2.
+Proof.
+  introv cl1 cl2 ext.
+  repeat unflsubst.
+  apply eq_lsubst_aux_if_ext_eq; eauto 3 with slow;
+  rw @sub_free_vars_if_cl_sub; auto.
+Qed.
+
+Lemma implies_closed_sub_find_def {o} :
+  forall (s : @Sub o) v d,
+    closed d
+    -> cl_sub s
+    -> closed (sub_find_def s v d).
+Proof.
+  introv ispd isps.
+  unfold sub_find_def.
+  remember (sub_find s v) as sf; destruct sf; symmetry in Heqsf; auto.
+  apply sub_find_some in Heqsf.
+  rw @cl_sub_eq in isps.
+  apply in_sub_eta in Heqsf; repnd.
+  apply isps in Heqsf; eauto 3 with slow.
+Qed.
+Hint Resolve implies_closed_sub_find_def : slow.
+
+Lemma prog_sub_sub_keep {o} :
+  forall (s : @Sub o) vs, prog_sub s -> prog_sub (sub_keep s vs).
+Proof.
+  induction s; introv ps; allsimpl; auto.
+  destruct a; boolvar; allsimpl; auto;
+  allrw @prog_sub_cons; repnd; dands; eauto 3 with slow.
+Qed.
+Hint Resolve prog_sub_sub_keep : slow.
+
+Lemma in_dom_sub_sub_keep_implies {o} :
+  forall (sub : @Sub o) vs v,
+    LIn v (dom_sub (sub_keep sub vs))
+    <=> (LIn v vs # LIn v (dom_sub sub)).
+Proof.
+  induction sub; split; introv i; repnd; allsimpl; tcsp.
+  - boolvar; allsimpl; repndors; subst; tcsp; apply IHsub in i; sp.
+  - boolvar; allsimpl; repndors; subst; tcsp.
+    + right; apply IHsub; sp.
+    + apply IHsub; sp.
+Qed.
+
+Lemma implies_isprog_sub_find_def {o} :
+  forall (s : @Sub o) v d,
+    isprog d
+    -> prog_sub s
+    -> isprog (sub_find_def s v d).
+Proof.
+  introv ispd isps.
+  unfold sub_find_def.
+  remember (sub_find s v) as sf; destruct sf; symmetry in Heqsf; auto.
+  apply sub_find_some in Heqsf.
+  rw <- @prog_sub_eq in isps.
+  apply in_sub_eta in Heqsf; repnd.
+  apply isps in Heqsf; eauto 3 with slow.
+Qed.
+Hint Resolve implies_isprog_sub_find_def : slow.
+
+Lemma prog_sub_sub_select {o} :
+  forall (s : @Sub o) d vs,
+    isprog d
+    -> prog_sub s
+    -> prog_sub (sub_select s vs d).
+Proof.
+  induction vs; introv pd ps; allsimpl; eauto 3 with slow.
+  apply prog_sub_cons; dands; auto.
+  destruct a; boolvar; allsimpl; auto;
+  allrw @prog_sub_cons; repnd; dands; eauto 3 with slow.
+Qed.
+Hint Resolve prog_sub_sub_select : slow.
+
+Lemma sub_find_sub_select {o} :
+  forall (s : @Sub o) vs d v,
+    sub_find (sub_select s vs d) v
+    = if memvar v vs
+      then Some (sub_find_def s v d)
+      else None.
+Proof.
+  induction vs; introv; simpl; auto.
+  allrw memvar_cons; boolvar; tcsp.
+  - rw IHvs; boolvar; tcsp.
+  - rw IHvs; boolvar; tcsp.
+Qed.
+
+Lemma cl_sub_sub_select {o} :
+  forall (s : @Sub o) d vs,
+    closed d
+    -> cl_sub s
+    -> cl_sub (sub_select s vs d).
+Proof.
+  induction vs; introv pd ps; allsimpl; eauto 3 with slow.
+  apply cl_sub_cons; dands; auto.
+  destruct a; boolvar; allsimpl; auto;
+  allrw @cl_sub_cons; repnd; dands; eauto 3 with slow.
+Qed.
+Hint Resolve cl_sub_sub_select : slow.
+
+Lemma cl_lsubst_trim_select {o} :
+  forall t (sub : @Sub o) lv d,
+    cl_sub sub
+    -> closed d
+    -> (forall v, LIn v (free_vars t) -> (LIn v lv <=> LIn v (dom_sub sub)))
+    -> lsubst t sub = lsubst t (sub_select sub lv d).
+Proof.
+  introv cls cld sv.
+  apply cl_eq_lsubst_if_ext_eq; eauto 3 with slow.
+  introv i.
+  applydup sv in i.
+  rw @sub_find_sub_select.
+  unfold sub_find_def.
+  boolvar.
+  - applydup i0 in Heqb.
+    apply in_dom_sub_exists in Heqb0; exrepnd.
+    rw Heqb1; simpl; auto.
+  - rw @sub_find_none_if; simpl; auto.
+    intro h.
+    apply i0 in h; sp.
+Qed.
+
+Lemma isvalue_like_lam {o} :
+  forall v (t : @NTerm o), isvalue_like (mk_lam v t).
+Proof.
+  introv.
+  unfold isvalue_like; simpl; tcsp.
+Qed.
+Hint Resolve isvalue_like_lam : slow.
+
+Lemma cl_olift_iff_pv_olift {o} :
+  forall R (x y : @NTerm o) vs,
+    isprog_vars vs x
+    -> isprog_vars vs y
+    -> (pv_olift R x y vs <=> cl_olift R x y).
+Proof.
+  introv ispx ispy.
+  unfold pv_olift, cl_olift.
+  split; intro h; repnd; dands; eauto 3 with slow.
+
+  - introv ps isp1 isp2.
+    applydup @lsubst_program_implies in isp1.
+    applydup @lsubst_program_implies in isp2.
+    applydup @isprog_vars_eq in ispx; repnd.
+    applydup @isprog_vars_eq in ispy; repnd.
+    allrw @subvars_eq.
+
+    pose proof (h (sub_select sub vs mk_axiom)) as q; clear h.
+    rw @dom_sub_sub_select in q.
+    repeat (autodimp q hyp); eauto 2 with slow.
+
+    rw <- @cl_lsubst_trim_select in q; eauto 2 with slow;
+    [|introv i;applydup isp0 in i;apply ispx1 in i; sp].
+
+    rw <- @cl_lsubst_trim_select in q; eauto 2 with slow.
+    introv i;applydup isp3 in i;apply ispy1 in i; sp.
+
+  - introv ps e.
+    apply h; auto.
+
+    + apply isprogram_lsubst_if_isprog_sub; eauto 2 with slow.
+      introv i.
+      apply isprog_vars_eq in ispx; repnd.
+      allrw subvars_eq.
+      apply ispx0 in i; subst; sp.
+
+    + apply isprogram_lsubst_if_isprog_sub; eauto 2 with slow.
+      introv i.
+      apply isprog_vars_eq in ispy; repnd.
+      allrw subvars_eq.
+      apply ispy0 in i; subst; sp.
+Qed.
+
+Lemma implies_approxc_lam {o} :
+  forall lib v (t1 t2 : @CVTerm o [v]),
+    (forall u : CTerm, cequivc lib (substc u v t1) (substc u v t2))
+    -> approxc lib (mkc_lam v t1) (mkc_lam v t2).
+Proof.
+  introv imp.
+  destruct_cterms.
+  allunfold @cequivc; allsimpl.
+  allunfold @approxc; allsimpl.
+
+  constructor.
+  unfold close_comput; dands;
+  try (apply isprogram_lam);
+  eauto 3 with slow.
+
+  + introv comp.
+    apply computes_to_value_isvalue_eq in comp;
+      try (apply isvalue_mk_lam); eauto 3 with slow.
+    unfold mk_lam in comp; ginv; fold_terms.
+    exists [bterm [v] x]; fold_terms.
+    dands.
+    { apply computes_to_value_isvalue_refl;
+      try (apply isvalue_mk_lam); eauto 3 with slow. }
+
+    unfold lblift; simpl; dands; auto.
+    introv ltn.
+    destruct n; try omega; clear ltn.
+    unfold selectbt; simpl.
+    unfold blift.
+    exists [v] x0 x; dands; eauto 3 with slow.
+    apply clearbots_olift.
+    apply cl_olift_implies_olift; eauto 3 with slow.
+
+    pose proof (cl_olift_iff_pv_olift (approx lib) x0 x [v]) as xx.
+    repeat (autodimp xx hyp).
+    apply xx; clear xx.
+    introv ps e.
+    destruct sub as [|p s]; allsimpl; ginv.
+    destruct s; ginv.
+    destruct p as [z u]; allsimpl.
+    allrw @fold_subst.
+    allrw @prog_sub_cons; repnd.
+    pose proof (imp (mk_cterm u ps0)) as h; clear imp; allsimpl.
+    destruct h; sp.
+
+  + introv comp.
+    apply can_doesnt_raise_an_exception in comp; sp.
+
+  + introv comp.
+    apply reduces_to_if_isvalue_like in comp; ginv; eauto 3 with slow.
+Qed.
+
+Lemma cequivc_iff_approxc {o} :
+  forall lib (a b : @CTerm o),
+    cequivc lib a b <=> (approxc lib a b # approxc lib b a).
+Proof.
+  introv; destruct_cterms; unfold cequivc, approxc; simpl; sp.
+Qed.
+
+Lemma implies_cequivc_lam {o} :
+  forall lib v (t1 t2 : @CVTerm o [v]),
+    (forall u : CTerm, cequivc lib (substc u v t1) (substc u v t2))
+    -> cequivc lib (mkc_lam v t1) (mkc_lam v t2).
+Proof.
+  introv imp.
+  apply cequivc_iff_approxc; dands.
+  - apply implies_approxc_lam; auto.
+  - apply implies_approxc_lam; auto.
+    introv.
+    apply cequivc_sym; auto.
+Qed.
+
+Lemma implies_approx_lam2 {o} :
+  forall lib v1 v2 (t1 t2 : @NTerm o),
+    isprog_vars [v1] t1
+    -> isprog_vars [v2] t2
+    -> (forall u : NTerm, isprog u -> cequiv lib (subst t1 v1 u) (subst t2 v2 u))
+    -> approx lib (mk_lam v1 t1) (mk_lam v2 t2).
+Proof.
+  introv isp1 isp2 imp.
+
+  constructor.
+  unfold close_comput; dands;
+  try (apply isprogram_lam);
+  eauto 3 with slow.
+
+  - introv comp.
+    apply computes_to_value_isvalue_eq in comp;
+      try (apply isvalue_mk_lam); eauto 3 with slow.
+    unfold mk_lam in comp; ginv; fold_terms.
+    exists [bterm [v2] t2]; fold_terms.
+    dands.
+    { apply computes_to_value_isvalue_refl;
+      try (apply isvalue_mk_lam); eauto 3 with slow. }
+
+    unfold lblift; simpl; dands; auto.
+    introv ltn.
+    destruct n; try omega; clear ltn.
+    unfold selectbt; simpl.
+    unfold blift.
+    exists [v1] t1 (subst t2 v2 (mk_var v1)); dands; eauto 3 with slow.
+
+    + apply clearbots_olift.
+      apply cl_olift_implies_olift; eauto 3 with slow.
+
+      pose proof (cl_olift_iff_pv_olift (approx lib) t1 (subst t2 v2 (mk_var v1)) [v1]) as xx.
+      repeat (autodimp xx hyp).
+      { clear imp; allrw @isprog_vars_eq; repnd; dands.
+        - eapply subvars_eqvars;
+          [|apply eqvars_sym;apply eqvars_free_vars_disjoint].
+          simpl.
+          rw subvars_app_l; dands.
+          + apply subvars_remove_nvars; simpl.
+            eapply subvars_trans;eauto.
+            rw subvars_prop; simpl; tcsp.
+          + boolvar; simpl; eauto 3 with slow.
+        - apply nt_wf_subst; eauto 3 with slow. }
+      apply xx; clear xx.
+      introv ps e.
+      destruct sub as [|p s]; allsimpl; ginv.
+      destruct s; ginv.
+      destruct p as [z u]; allsimpl.
+      allrw @fold_subst.
+      allrw @prog_sub_cons; repnd.
+      pose proof (imp u) as h; clear imp; allsimpl.
+      autodimp h hyp; eauto 3 with slow.
+      destruct h; sp.
+      eapply approx_trans; eauto.
+
+      eapply approx_alpha_rw_r_aux;
+        [apply alpha_eq_sym;apply combine_sub_nest|].
+      simpl.
+      allrw @fold_subst.
+      rw @subst_mk_var1.
+
+      destruct (deq_nvar v2 z); subst.
+
+      * pose proof (cl_lsubst_app_sub_filter t2 [(z,u)] [(z,u)]) as h; allsimpl.
+        autodimp h hyp; eauto 3 with slow.
+        allrw memvar_singleton; boolvar; rw h; eauto 3 with slow.
+
+      * pose proof (lsubst_sub_filter_alpha t2 [(v2, u), (z, u)] [z]) as h.
+        allrw disjoint_singleton_r; allsimpl.
+        allrw memvar_singleton; boolvar; tcsp.
+        autodimp h hyp.
+        { allrw @isprog_vars_eq; repnd.
+          allrw subvars_eq.
+          introv h; apply isp0 in h; allsimpl; tcsp. }
+
+        eapply approx_alpha_rw_r_aux;[exact h|].
+        allrw @fold_subst; eauto 3 with slow.
+
+    + pose proof (alpha_eq_bterm_single_change t2 v2) as h.
+      allrw subset_singleton_r.
+      autodimp h hyp.
+      { introv ix.
+        clear imp.
+        allrw @isprog_vars_eq; repnd.
+        allrw subvars_eq.
+        apply isp3 in ix; allsimpl; tcsp. }
+      apply h.
+
+  - introv comp.
+    apply can_doesnt_raise_an_exception in comp; sp.
+
+  - introv comp.
+    apply reduces_to_if_isvalue_like in comp; ginv; eauto 3 with slow.
+Qed.
+
+Lemma implies_approxc_lam2 {o} :
+  forall lib v1 v2 (t1 : @CVTerm o [v1]) t2,
+    (forall u : CTerm, cequivc lib (substc u v1 t1) (substc u v2 t2))
+    -> approxc lib (mkc_lam v1 t1) (mkc_lam v2 t2).
+Proof.
+  introv imp.
+  destruct_cterms.
+  allunfold @cequivc; allsimpl.
+  allunfold @approxc; allsimpl.
+
+  apply implies_approx_lam2; auto.
+  introv isp.
+  apply isprogram_eq in isp.
+  pose proof (imp (mk_cterm u isp)) as k; allsimpl; auto.
+Qed.
+
+Lemma implies_cequivc_lam2 {o} :
+  forall lib v1 v2 (t1 : @CVTerm o [v1]) t2,
+    (forall u : CTerm, cequivc lib (substc u v1 t1) (substc u v2 t2))
+    -> cequivc lib (mkc_lam v1 t1) (mkc_lam v2 t2).
+Proof.
+  introv imp.
+  apply cequivc_iff_approxc; dands.
+  - apply implies_approxc_lam2; auto.
+  - apply implies_approxc_lam2; auto.
+    introv.
+    apply cequivc_sym; auto.
+Qed.
+
+Lemma nt_wf_lambda_iff {p} :
+  forall (bs : list (@BTerm p)),
+    nt_wf (oterm (Can NLambda) bs)
+    <=> {v : NVar
+        $ {b : NTerm
+        $ bs = [bterm [v] b]
+        # nt_wf b}}.
+Proof.
+  introv; split; intro k.
+  - inversion k as [|?|? ? imp e]; clear k; subst.
+    allsimpl.
+    repeat (destruct bs; allsimpl; ginv).
+    destruct b as [l1 t1].
+    allunfold @num_bvars; allsimpl.
+    repeat (destruct l1; ginv).
+    pose proof (imp (bterm [n] t1)) as h1.
+    autodimp h1 hyp.
+    clear imp.
+    allrw @bt_wf_iff.
+    exists n t1; dands; auto.
+  - exrepnd; subst.
+    repeat constructor.
+    introv i; allsimpl; repndors; subst; tcsp.
+Qed.
+
+
+(*
+*** Local Variables:
+*** coq-load-path: ("." "../util/" "../terms/" "../computation/")
+*** End:
+*)
