per/sequents2.v
@@ -1,0 +1,88 @@
+(*
+
+  Copyright 2014 Cornell University
+  Copyright 2015 Cornell University
+
+  This file is part of VPrl (the Verified Nuprl project).
+
+  VPrl is free software: you can redistribute it and/or modify
+  it under the terms of the GNU General Public License as published by
+  the Free Software Foundation, either version 3 of the License, or
+  (at your option) any later version.
+
+  VPrl is distributed in the hope that it will be useful,
+  but WITHOUT ANY WARRANTY; without even the implied warranty of
+  MERCHANTABILITY or FITNESS FOR A PARTICULAR PURPOSE.  See the
+  GNU General Public License for more details.
+
+  You should have received a copy of the GNU General Public License
+  along with VPrl.  If not, see <http://www.gnu.org/licenses/>.
+
+
+  Website: http://nuprl.org/html/verification/
+  Authors: Abhishek Anand & Vincent Rahli
+
+*)
+
+Require Export sequents.
+
+Definition wf_bseq {o} (s : @baresequent o) :=
+  vswf_hypotheses [] (hyps s)
+  # wf_term (ctype (concl s))
+  # closed_type_baresequent s.
+
+(* This is a variant of [rule_true2] (which is equivalent to [rule_true])
+   that only needs [wf_bseq] and not [pwf_sequent].
+ *)
+Definition rule_true3 {o} lib (R : @rule o) : Type :=
+  forall wf    : wf_bseq (goal R),
+  forall cargs : args_constraints (sargs R) (hyps (goal R)),
+  forall hyps  : (forall s, LIn s (subgoals R) -> sequent_true2 lib s),
+    sequent_true2 lib (goal R).
+
+Lemma pwf_sequent_implies_wf_bseq {o} :
+  forall (seq : @baresequent o),
+    pwf_sequent seq -> wf_bseq seq.
+Proof.
+  introv wf.
+  unfold pwf_sequent, wf_sequent, wf_concl in wf; unfold wf_bseq; repnd; dands; auto.
+Qed.
+Hint Resolve pwf_sequent_implies_wf_bseq : slow.
+
+(* The other direction is not true because [rule_true] and [rule_true2] assume
+   that the extract is well-formed. *)
+Lemma rule_true3_implies_rule_true2 {o} :
+  forall lib (R : @rule o), rule_true3 lib R -> rule_true2 lib R.
+Proof.
+  introv rt wf args imp.
+  unfold rule_true3 in rt.
+  repeat (autodimp rt hyp); eauto 3 with slow.
+Qed.
+Hint Resolve rule_true3_implies_rule_true2 : slow.
+
+Lemma rule_true3_implies_rule_true {o} :
+  forall lib (R : @rule o), rule_true3 lib R -> rule_true lib R.
+Proof.
+  introv rt.
+  rw @rule_true_iff_rule_true2; eauto 3 with slow.
+Qed.
+Hint Resolve rule_true3_implies_rule_true : slow.
+
+Definition wf_subgoals2 {o} (R : @rule o) :=
+  forall s, LIn s (subgoals R) -> wf_bseq s.
+
+Lemma fold_wf_subgoals2 {o} :
+  forall R : @rule o,
+    (forall s, LIn s (subgoals R) -> wf_bseq s) = wf_subgoals2 R.
+Proof. sp. Qed.
+
+(* This is a variant of [wf_rule] that uses [wf_bseq] instead of [pwf_sequent] *)
+Definition wf_rule2 {o} (R : @rule o) :=
+  wf_bseq (goal R) -> wf_subgoals2 R.
+
+
+(*
+*** Local Variables:
+*** coq-load-path: ("." "../util/" "../terms/" "../computation/" "../cequiv/" "../close/")
+*** End:
+*)
